lunarlander_sl/Repetition.thy
@@ -5,15 +5,15 @@ begin
 subsection \<open>Alternative rule for repetition\<close>
 
 theorem Valid_frame:
-  assumes "Valid (\<lambda>s tr. P s \<and> tr = []) c (\<lambda>s tr. Q s \<and> R tr)"
-  shows "Valid (\<lambda>s tr. P s \<and> R' tr) c (\<lambda>s tr. Q s \<and> (R' @\<^sub>t R) tr)"
+  assumes "\<Turnstile> {\<lambda>s tr. P s \<and> tr = []} c {\<lambda>s tr. Q s \<and> R tr}"
+  shows "\<Turnstile> {\<lambda>s tr. P s \<and> R' tr} c {\<lambda>s tr. Q s \<and> (R' @\<^sub>t R) tr}"
   using assms unfolding Valid_def
   by (auto simp add: join_assn_def)
 
 theorem Valid_loop2:
   assumes "\<And>a tr1 tr2. Q a tr1 \<Longrightarrow> P (f a) tr2 \<Longrightarrow> P a (tr1 @ tr2)"
-    and "\<And>a. Valid (\<lambda>s tr. R a s \<and> tr = []) c (\<lambda>s tr. R (f a) s \<and> Q a tr)"
-  shows "Valid (\<lambda>s tr. \<exists>b. R b s \<and> (P b @- P a) tr) c (\<lambda>s tr. \<exists>b. R b s \<and> (P b @- P a) tr)"
+    and "\<And>a. \<Turnstile> {\<lambda>s tr. R a s \<and> tr = []} c {\<lambda>s tr. R (f a) s \<and> Q a tr}"
+  shows "\<Turnstile> {\<lambda>s tr. \<exists>b. R b s \<and> (P b @- P a) tr} c {\<lambda>s tr. \<exists>b. R b s \<and> (P b @- P a) tr}"
   apply (rule Valid_ex_pre)
   subgoal for b
     apply (rule Valid_ex_post) apply (rule exI[where x="f b"])
@@ -26,8 +26,8 @@ theorem Valid_loop2:
 theorem Valid_loop3:
   assumes "\<And>a. P a []"
   assumes "\<And>a tr1 tr2. Q a tr1 \<Longrightarrow> P (f a) tr2 \<Longrightarrow> P a (tr1 @ tr2)"
-    and "\<And>a. Valid (\<lambda>s tr. R a s \<and> tr = []) c (\<lambda>s tr. R (f a) s \<and> Q a tr)"
-  shows "Valid (\<lambda>s tr. R a s \<and> tr = []) (Rep c) (\<lambda>s tr. \<exists>b. R b s \<and> P a tr)"
+    and "\<And>a. \<Turnstile> {\<lambda>s tr. R a s \<and> tr = []} c {\<lambda>s tr. R (f a) s \<and> Q a tr}"
+  shows "\<Turnstile> {\<lambda>s tr. R a s \<and> tr = []} Rep c {\<lambda>s tr. \<exists>b. R b s \<and> P a tr}"
   apply (rule Valid_weaken_pre)
   prefer 2 apply (rule Valid_strengthen_post)
     prefer 2 apply (rule Valid_rep[where P="\<lambda>s tr. \<exists>b. R b s \<and> (P b @- P a) tr"])
